examples/csl/SL.Base.fst
@@ -3,3 +3,4 @@ module SL.Base
 include SL.Heap
 include SL.Effect
 include SL.Actions
+include SL.ConcurrentActions
