examples/csl/SL.ConcurrentActions.fst
@@ -1,0 +1,109 @@
+module SL.ConcurrentActions
+
+open SL.Heap
+open SL.Effect
+
+let par_comp #a #b (wpa : st_wp a) (wpb : st_wp b) post m1 m2 =
+   defined (m1 <*> m2) ==> 
+   wpa (fun a m1' -> wpb (fun b m2' -> defined (m1' <*> m2') /\ post (a, b) (m1' <*> m2')) m2) m1
+        
+let par_wp' #a #b (wpa : st_wp a) (wpb : st_wp b) post m =
+    exists m1 m2.
+           defined (m1 <*> m2)
+        /\ m == (m1 <*> m2)
+        /\ par_comp wpa wpb post m1 m2
+
+(* Silly lemma, but allows to handle goals properly *)
+let par_wp'_lemma
+  #a #b
+  (#wpa : st_wp a)
+  (#wpb : st_wp b)
+  (m m1 m2 : memory)
+  (post : post (a * b))
+  (_ : squash (defined (m1 <*> m2)))
+  (_ : squash (m == (m1 <*> m2)))
+  (_ : squash (par_comp wpa wpb post m1 m2))
+  //(_ : squash (wpa (fun a m1' -> forall b. post (a, b) m1') m1))
+  //(_ : squash (wpb (fun b m2' -> forall a. post (a, b) m2') m2))
+     : Lemma (defined (m1 <*> m2)
+               /\ m == (m1 <*> m2)
+               /\ (par_comp wpa wpb post m1 m2)) = ()
+
+let frame_wp_lemma (#a:Type) (#wp:st_wp a) (#f_post:memory -> post a) (m m0 m1:memory)
+    (_ : squash ((m0 <*> m1) == m))
+    (_ : squash (defined m))
+    (_ : squash (wp (f_post m1) m0)) :
+         (squash (frame_wp wp f_post m)) = ()
+
+let par_wp #a #b (wpa : st_wp a) (wpb : st_wp b) : st_wp (a * b) =
+  fun post m0 -> frame_wp (par_wp' wpa wpb) (frame_post post) m0
+
+assume val par : (#a:Type) -> (#b:Type) ->
+                 (#wpa : st_wp a) ->  (#wpb : st_wp b) ->
+                 ($f : (unit -> STATE a wpa)) ->
+                 ($g : (unit -> STATE b wpb)) ->
+                 STATE (a * b) (par_wp wpa wpb)
+
+
+
+(* Locks and operations *)
+// Locks are over a particular reference r.
+// Can we use a list or a set? Non-trivial to make it work. Even a set of addresses causes many blowups.
+// Can we use a heap predicate? Can we automate frame inference then?
+assume new type lock : #a:Type -> ref a -> Type0
+
+let mklock_wp #a (r:ref a) post m = exists v. m == r |> v /\ (forall (l:lock r). post l emp)
+let frame_mklock_wp r post m0 = frame_wp (mklock_wp r) (frame_post post) m0
+assume val mklock : #a:Type -> (r: ref a) ->
+                    STATE (lock r) (frame_mklock_wp r)
+
+  //let l = mklock r in
+  //acquire l;
+  //par (fun () -> acquire l; r := 2; release l)
+  //    (fun () -> r := !r + 1; release l)
+
+
+let acquire_wp r l post m = m == emp /\ (forall v. post () (r |> v))
+let frame_acquire_wp r l post m0 = frame_wp (with_fp [] <| acquire_wp r l) (frame_post post) m0
+assume val acquire : #a:Type -> (#r: ref a) -> (l : lock r) ->
+                     STATE unit (frame_acquire_wp r l)
+
+
+let release_wp r l post m = (exists v. m == r |> v) /\ post () emp
+let frame_release_wp r l post m0 = frame_wp (with_fp [tosref r] <| release_wp r l) (frame_post post) m0
+assume val release : #a:Type -> (#r: ref a) -> (l : lock r) ->
+                     STATE unit (frame_release_wp r l)
+
+
+// let locking_wp r l wp post m =
+//     wp (fun x m' -> forall v m1. m' == (r |> v <*> m1) ==> post x m1) m
+// 
+// assume val locking : #a:Type -> #b:Type -> #r:(ref a) -> (l : lock r) ->
+//                      (#wp : st_wp b) -> (f : unit -> STATE b wp) ->
+//                   STATE b (frame_locking_wp r l wp)
+
+
+(* A version with explicit heaps *)
+unfold let par_wp'_exp #a #b (wpa : st_wp a) (wpb : st_wp b) (m1 m2 : memory)
+                       (post : post (a * b)) (m : memory) : Type0 =
+         defined (m1 <*> m2)
+        /\ m == (m1 <*> m2)
+        /\ wpa (fun a m1' -> wpb (fun b m2' -> post (a, b) (m1' <*> m2')) m2) m1
+
+let par_wp_exp #a #b (wpa : st_wp a) (wpb : st_wp b) (m1 m2 : memory) : st_wp (a * b) =
+  fun post m0 -> frame_wp (par_wp'_exp wpa wpb m1 m2) (frame_post post) m0
+
+assume val par_exp : (#a:Type) -> (#b:Type) ->
+                 (#wpa : st_wp a) ->  (#wpb : st_wp b) ->
+                 (m1 : memory) -> (m2 : memory) ->
+                 ($f : (unit -> STATE a wpa)) ->
+                 ($g : (unit -> STATE b wpb)) ->
+                 STATE (a * b) (par_wp_exp #a #b wpa wpb m1 m2)
+
+(* Unframed, explicit variant. Not very user-friendly. *)
+assume val par_exp' : (#a:Type) -> (#b:Type) ->
+                 (#wpa : st_wp a) ->  (#wpb : st_wp b) ->
+                 (m1 : memory) -> (m2 : memory) ->
+                 ($f : (unit -> STATE a wpa)) ->
+                 ($g : (unit -> STATE b wpb)) ->
+                 STATE (a * b) (par_wp'_exp #a #b wpa wpb m1 m2)
