examples/csl/SL.ConcurrentExamples.fst
@@ -1,0 +1,91 @@
+module SL.ConcurrentExamples
+
+open SL.Heap
+open SL.Effect
+open SL.ConcurrentActions
+open SL.AutoTactic
+
+// Lift from PURE to STATE, needed since we use $ for some args, which is annoying...
+let l (x:'a) : STATE 'a (fun p m -> m == emp /\ p x m) = x
+
+(* A trivial test without mentioning heaps *)
+//let test03 (r:ref int) : ST int (fun p m -> exists v. m == r |> v /\ p 3 (r |> v)) by (sl_auto ())
+//=
+//  let (x, y) = par (fun () -> l 1) (fun () -> l 2) in
+//  x + y
+
+
+(* Actually changing a reference *)
+//let test04 (r:ref int) : ST int (fun p m -> exists v. m == r |> v /\ p 3 (r |> v)) by (sl_auto ())
+//=
+//  let (x, y) = par // #_ #_ #(bind_wp (range_of ()) _ _ (frame_write_wp r 2) (fun _ -> return_wp _ 1)) #_
+//                 (fun () -> r := 2; 1) (fun () -> l 2) in
+//  x + y
+
+let noaddrs = Set.empty #nat
+
+  //#set-options "--print_full_names"
+
+#set-options "--debug SL.ConcurrentExamples"
+
+
+// let addrs_emp (m m':memory) : Lemma (requires (defined m /\ addrs_in m == Set.empty))
+//                                  (ensures (defined (m <*> m') /\ m <*> m' == m'))
+//                                  [SMTPat (m <*> m')] // TODO: very likely a bad pattern
+//      = admit () // provable from inside SL.Heap
+
+let test05' (r:ref int) (l:lock r) : ST int (fun p m -> m == emp /\ (forall v. p 3 (r |> v))) [tosref r] by (sl_auto ())
+                            
+  =
+  acquire l;
+  3
+
+let test05 (r:ref int) (l:lock r) : ST unit (fun p m -> m == emp /\ p () emp) [] by (sl_auto ())
+                            
+  =
+  acquire l;
+  //let v = !r in
+  release l
+
+
+
+
+
+let test06 (r:ref int) : ST int (fun p m -> exists v. m == r |> v /\ p 3 (r |> v)) by (sl_auto ()) =
+  let l = mklock (fun p -> True) in
+  let _ = par (fun () -> acquire l; release l; 1) (fun () -> acquire l; release l; 2) in
+  3
+
+unfold let return_wp (a:Type) (x:a) :st_wp a = 
+  fun post m0 -> m0 == emp /\ post x m0
+
+open FStar.Tactics
+
+// `compute` is needed for these two, but they work without the tactic since they are
+// explicit about their heaps already. We also use STATE instead of the framed ST.
+let test01 () : STATE int (fun p m -> forall r. m == emp /\ p r m) by (compute ())
+=
+  let (x, y) = par_exp' emp emp (fun () -> l 1) (fun () -> l 2) in
+  x + y
+
+let test02 () : STATE int (fun p m -> m == emp /\ p 3 m) by (compute ())
+=
+  let (x, y) = par_exp' emp emp (fun () -> l 1) (fun () -> l 2) in
+  x + y
+
+(* Sanity check that other programs still work.. since we modified the tactic *)
+let swap_wp (r1 r2:ref int) = fun p m -> exists x y. m == (r1 |> x <*> r2 |> y) /\ p () (r1 |> y <*> r2 |> x)
+let swap (r1 r2:ref int) :ST unit (swap_wp r1 r2) by (sl_auto ())
+  = let x = !r1 in
+    let y = !r2 in
+    r1 := y;
+    r2 := x
+
+#set-options "--print_full_names --prn --print_implicits"
+
+(* This is explicit about the frames of the parallel composition, but still requires
+ * non-trivial frame reasoning *)
+let test03' (r:ref int) : ST int (fun p m -> exists v. m == r |> v /\ p 3 (r |> v)) by (sl_auto ())
+=
+  let (x, y) = par_exp emp emp (fun () -> l 1) (fun () -> l 2) in
+  x + y
